ZiskFv/Compliance/AddSpinWitness.lean
@@ -1034,7 +1034,6 @@ def addSpinAcceptedTrace : AcceptedZiskTrace 2 where
   mem_replay_im0 := fun h => absurd h addSpinWitness_not_mutableMemPresent
   mem_replay_im1 := fun h => absurd h addSpinWitness_not_mutableMemPresent
   mem_replay_constraints := fun h => absurd h addSpinWitness_not_mutableMemPresent
-  mem_replay_row_ranges := fun h => absurd h addSpinWitness_not_mutableMemPresent
   mem_replay_segment_ranges := fun h => absurd h addSpinWitness_not_mutableMemPresent
   mem_replay_source_covers := fun h => absurd h addSpinWitness_not_mutableMemPresent
   transitions_hold := addSpinWitness_transitions
@@ -1099,7 +1098,6 @@ def addPaddedAcceptedTrace : AcceptedZiskTrace 1 where
   mem_replay_im0 := fun h => absurd h addSpinWitness_not_mutableMemPresent
   mem_replay_im1 := fun h => absurd h addSpinWitness_not_mutableMemPresent
   mem_replay_constraints := fun h => absurd h addSpinWitness_not_mutableMemPresent
-  mem_replay_row_ranges := fun h => absurd h addSpinWitness_not_mutableMemPresent
   mem_replay_segment_ranges := fun h => absurd h addSpinWitness_not_mutableMemPresent
   mem_replay_source_covers := fun h => absurd h addSpinWitness_not_mutableMemPresent
   transitions_hold := addSpinWitness_transitions
